binary-search-tree: Qed.

binary-search-tree/BST.v
@@ -1,4 +1,5 @@
 Require Import Coq.Arith.Arith.
+Require Import Omega.
 
 (* This formalization of BST is slightly modified from 6.887's homework. *)
 
@@ -17,6 +18,8 @@ Fixpoint tree_gt_n (t : tree) (n : nat) : Prop :=
   | Leaf => True
   | Node v l r => v > n /\ tree_gt_n l n /\ tree_gt_n r n
   end.
+
+(* TODO: Merge tree_lt_n and tree_gt_n. *)
 
 Fixpoint BST (t : tree) : Prop :=
   match t with
@@ -47,12 +50,46 @@ Fixpoint member (t: tree) (n : nat) : bool :=
                   end
   end.
 
+Fixpoint leftmost (t: tree) : option nat :=
+  match t with
+  | Leaf => None
+  | Node v Leaf _ => Some v
+  | Node _ l _ => leftmost l
+  end.
+
+Fixpoint delete_leftmost (t : tree) : tree :=
+  match t with
+  | Leaf => Leaf
+  | Node _ Leaf r => r
+  | Node v l r => Node v (delete_leftmost l) r
+  end.
+
+Fixpoint delete (t : tree) (n : nat) : tree :=
+  match t with
+  | Leaf => Leaf
+  | Node v l r =>
+      match n ?= v with
+      | Lt => Node v (delete l n) r
+      | Gt => Node v l (delete r n)
+      | Eq => match l with
+              | Leaf => r
+              | _ => match leftmost r with
+                     | Some v' => Node v' l (delete_leftmost r) 
+                     | None => l
+                     end
+              end
+      end
+  end.
+
 Ltac unfold_tree :=
   repeat (
     unfold BST in *; fold BST in *;
     unfold tree_lt_n in *; fold tree_lt_n in *;
     unfold tree_gt_n in *; fold tree_gt_n in *;
-    unfold insert in *; fold insert in *
+    unfold insert in *; fold insert in *;
+    unfold leftmost in *; fold leftmost in *;
+    unfold delete_leftmost in *; fold delete_leftmost in *;
+    unfold delete in *; fold delete in *
   ).
 
 Ltac bool_to_prop :=
@@ -75,7 +112,7 @@ Proof.
     destruct (n ?= n0) eqn:H5; simpl; rewrite H5; auto.
 Qed.
 
-Lemma tree_lt_n_insert_preserve:
+Lemma tree_lt_n_insert_preserve :
   forall (t : tree) (n0 n : nat),
     tree_lt_n t n -> n0 < n -> tree_lt_n (insert t n0) n.
 Proof.
@@ -83,10 +120,10 @@ Proof.
   induction t; intros; unfold_tree.
   - auto.
   - propositional.
-    destruct (n0 ?= n) eqn:Heq; bool_to_prop; unfold_tree; auto.
+    destruct (n0 ?= n) eqn:H2; bool_to_prop; unfold_tree; auto.
 Qed.
 
-Lemma tree_gt_n_insert_preserve:
+Lemma tree_gt_n_insert_preserve :
   forall (t : tree) (n0 n : nat),
     tree_gt_n t n -> n < n0 -> tree_gt_n (insert t n0) n.
 Proof.
@@ -94,7 +131,7 @@ Proof.
   induction t; intros; unfold_tree.
   - auto.
   - propositional.
-    destruct (n0 ?= n) eqn:Heq; bool_to_prop; unfold_tree; auto.
+    destruct (n0 ?= n) eqn:H2; bool_to_prop; unfold_tree; auto.
 Qed.
 
 Theorem insert_correct :
@@ -109,4 +146,139 @@ Proof.
       apply tree_lt_n_insert_preserve; auto.
     + propositional; auto.
       apply tree_gt_n_insert_preserve; auto.
+Qed.
+
+Lemma tree_lt_trans :
+  forall (t : tree) (n n0 : nat),
+  tree_lt_n t n -> n < n0 -> tree_lt_n t n0.
+Proof.
+  intros t.
+  induction t; intros; unfold_tree; auto; try propositional; try omega; eauto.
+Qed.
+
+Lemma tree_gt_trans :
+  forall (t : tree) (n n0 : nat),
+  tree_gt_n t n -> n > n0 -> tree_gt_n t n0.
+Proof.
+  intros t.
+  induction t; intros; unfold_tree; auto; try propositional; try omega; eauto.
+Qed.
+
+Lemma leftmost_lt :
+  forall (t : tree) (n n0 : nat),
+  tree_lt_n t n -> leftmost t = Some n0 -> n0 < n.
+Proof.
+  intros t.
+  induction t; intros; unfold_tree.
+  - inversion H0.
+  - destruct t1.
+    + inversion H0. subst. propositional.
+    + apply IHt1; propositional.
+Qed.
+
+Lemma leftmost_gt :
+  forall (t : tree) (n n0 : nat),
+  tree_gt_n t n -> leftmost t = Some n0 -> n0 > n.
+Proof.
+  intros t.
+  induction t; intros; unfold_tree.
+  - inversion H0.
+  - destruct t1.
+    + inversion H0. subst. propositional.
+    + apply IHt1; propositional.
+Qed.
+
+(* With this lemma, we can get rid of delete_leftmost! *)
+Lemma delete_leftmost_is_delete :
+  forall (t : tree) (n : nat),
+  BST t -> leftmost t = Some n -> delete_leftmost t = delete t n.
+Proof.
+  intros t.
+  induction t; intros; unfold_tree.
+  - simpl. auto.
+  - destruct t1.
+    + inversion H0; clear H0. rewrite Nat.compare_refl. auto.
+    + assert (n0 < n).
+      { eapply leftmost_lt; eauto. propositional. }
+      rewrite nat_compare_lt in H1. rewrite H1.
+      assert (delete_leftmost (Node n1 t1_1 t1_2) = delete (Node n1 t1_1 t1_2) n0).
+      { apply IHt1. propositional. auto. }
+      rewrite H2. auto.
+Qed.
+
+Lemma tree_lt_n_delete_preserve :
+  forall (t : tree) (n0 n : nat),
+    BST t -> tree_lt_n t n -> tree_lt_n (delete t n0) n.
+Proof.
+  intros t.
+  induction t; intros; unfold_tree.
+  - auto.
+  - destruct (n0 ?= n) eqn:H1; bool_to_prop.
+    + destruct t1; propositional.
+      remember (Node n0 t1_1 t1_2) as t1. clear Heqt1.
+      destruct (leftmost t2) eqn:H7.
+      * assert (n2 < n1). { apply (leftmost_lt t2 n1 n2); auto. }
+        rewrite (delete_leftmost_is_delete t2 n2); auto.
+        unfold_tree. propositional. auto.
+      * auto.
+    + unfold_tree. propositional. auto.
+    + unfold_tree. propositional. auto.
+Qed.
+
+Lemma tree_gt_n_delete_preserve :
+  forall (t : tree) (n0 n : nat),
+    BST t -> tree_gt_n t n -> tree_gt_n (delete t n0) n.
+Proof.
+  intros t.
+  induction t; intros; unfold_tree.
+  - auto.
+  - destruct (n0 ?= n) eqn:H1; bool_to_prop.
+    + destruct t1; propositional.
+      remember (Node n0 t1_1 t1_2) as t1. clear Heqt1.
+      destruct (leftmost t2) eqn:H7.
+      * assert (n2 > n1). { apply (leftmost_gt t2 n1 n2); auto. }
+        rewrite (delete_leftmost_is_delete t2 n2); auto.
+        unfold_tree. propositional. auto.
+      * auto.
+    + unfold_tree. propositional. auto.
+    + unfold_tree. propositional. auto.
+Qed.
+
+Theorem delete_leftmost_gt_n :
+  forall (t : tree) (n n0 : nat),
+    BST t -> leftmost t = Some n0 -> tree_gt_n t n -> tree_gt_n (delete_leftmost t) n0.
+Proof.
+  intros t.
+  induction t; intros; unfold_tree.
+  - auto.
+  - destruct t1.
+    + inversion H0. subst. propositional.
+    + remember (Node n2 t1_1 t1_2) as t1. clear Heqt1.
+      unfold_tree.
+      assert (n1 < n). { propositional. eapply leftmost_lt; eauto. }
+      propositional.
+      * eapply IHt1; eauto.
+      * eapply tree_gt_trans; eauto.
+Qed.
+
+Theorem delete_correct :
+  forall (t : tree) (n : nat), BST t -> BST (delete t n).
+Proof.
+  intros t.
+  induction t; intros; unfold_tree.
+  - simpl. auto.
+  - destruct (n0 ?= n) eqn:H1; bool_to_prop; unfold_tree.
+    + destruct t1.
+      * propositional.
+      * { destruct (leftmost t2) eqn:H1.
+          - remember (Node n0 t1_1 t1_2) as t1. clear Heqt1.
+            unfold_tree. propositional.
+            + rewrite (delete_leftmost_is_delete t2 n1); auto.
+            + assert (n1 > n). { eapply leftmost_gt. apply H4. apply H1. }
+              eapply tree_lt_trans. eauto. omega.
+            + eapply delete_leftmost_gt_n; eauto.
+          - propositional.
+        }
+    + propositional. auto. apply tree_lt_n_delete_preserve; auto.
+    + propositional. auto. apply tree_gt_n_delete_preserve; auto.
 Qed.
